assembly/64bits/extern.cpp
@@ -1,30 +1,42 @@
 #include <iostream>
+#include <assert.h>
 
 using namespace std;
 
-extern "C" long longASMFunction
-(
- long x1,
- long x2,
- long x3,
- long x4,
- long x5,
- long x6
- );
+#define LONG(n) 0x##n##n##n##n##n##n##n##n##n##n##n##n##n##n##n##n##UL
+
+// simply returns argument of given index 1-8
+extern "C" unsigned long 
+longASMFunction(
+    int index, 
+    unsigned long x1, 
+    unsigned long x2, 
+    unsigned long x3, 
+    unsigned long x4, 
+    unsigned long x5, 
+    unsigned long x6, 
+    unsigned long x7, 
+    unsigned long x8
+);
 
 int main()
 {
+  unsigned long x[] = {
+    LONG(1),    // 0x1111111111111111L
+    LONG(2),    // 0x2222222222222222L
+    LONG(3),    // 0x3333333333333333L
+    LONG(4),    // 0x4444444444444444L
+    LONG(5),    // 0x5555555555555555L
+    LONG(6),    // 0x6666666666666666L
+    LONG(7),    // 0x7777777777777777L
+    LONG(8)     // 0x8888888888888888L
+  };
 
-  long x1 = 0x1111111111111111L;
-  long x2 = 0x2222222222222222L;
-  long x3 = 0x3333333333333333L;
-  long x4 = 0x4444444444444444L;
-  long x5 = 0x5555555555555555L;
-  long x6 = 0x6666666666666666L;
+  cout << "\nAssembly function call from C++ with longs ...\n";
+  for(int i = 0; i < 8; ++i) {
+    cout << "x" << i + 1 << " = 0x" << hex << x[i] << endl;
+    assert(x[i] == longASMFunction(i+1,x[0],x[1],x[2],x[3],x[4],x[5],x[6],x[7]));
+  }
 
-  long res = longASMFunction(x1, x2, x3, x4, x5, x6);
-
-  cout << hex << "Result = 0x" << res << endl;
-  
   return 0;
 }
