assembly/hacking/hacking-network.h
@@ -1,0 +1,19 @@
+#ifndef INCLUDE_HACKING_NETWORK_H
+#define INCLUDE_HACKING_NETWORK_H
+
+/* This function accepts a socket FD and a ptr to the null terminated
+ * string to send. The function will make sure all the bytes of the
+ * string are sent. Returns 1 on success and 0 on failure.
+ */ 
+int send_string(int sockfd, const unsigned char *buffer);
+
+
+/* This function accepts a socket FD and a ptr to a destination
+ * buffer. It will receive from the socket until the EOL byte
+ * sequence in seen. The EOL bytes are read from the socket, but
+ * the destination buffer is terminated before these bytes.
+ * Returns the size of the read line (without EOL bytes). 
+ */ 
+int recv_line(int sockfd, unsigned char *dest_buffer); 
+
+#endif
