coq/logic.v
@@ -6,7 +6,6 @@ Inductive P (V : Set) : Set :=
   | Imply  : P V -> P V -> P V 
   | Forall : V -> P V -> P V.
 
-
 Fixpoint subst {V:Set}{W:Set} (sig: V -> W) (phi: P V) : P W :=
   match phi with
     | Belong x y        => Belong (sig x) (sig y)
@@ -22,26 +21,66 @@ Lemma subst_compose: forall U V W: Set,
   forall tau: U->V, forall sig: V->W, forall phi: P U, 
   subst (compose tau sig) phi = compose (subst tau) (subst sig) phi.
 
-  Proof.
+Proof.
   intros U V W tau sig phi. elim phi.
 
-  clear phi. intros x y. unfold subst at 1. unfold compose at 3.
-  unfold subst at 2. unfold subst at 1. unfold compose. reflexivity.
+  clear phi. intros x y. 
+    unfold subst at 1. unfold compose at 3.
+    unfold subst at 2. unfold subst at 1. unfold compose. 
+  reflexivity.
 
-  clear phi. unfold subst at 1. unfold compose. unfold subst at 2. 
-  unfold subst. reflexivity.
+  clear phi. 
+    unfold subst at 1. unfold compose. unfold subst at 2. 
+    unfold subst. 
+  reflexivity.
 
-  clear phi. intros p1 H1 p2 H2. unfold subst at 1.
-  fold (subst (compose tau sig) p1). fold (subst (compose tau sig) p2).
-  unfold compose at 3. unfold subst at 4. 
-  fold (subst tau p1). fold (subst tau p2). unfold subst at 3.
-  fold (subst sig (subst tau p1)). fold (subst sig (subst tau p2)).
-  fold (compose (subst tau) (subst sig) p1).
-  fold (compose (subst tau) (subst sig) p2).
-  rewrite <- H1. rewrite <- H2. reflexivity.
+  clear phi. intros p1 H1 p2 H2. 
+    unfold subst at 1.
+    fold (subst (compose tau sig) p1). 
+    fold (subst (compose tau sig) p2).
+    unfold compose at 3. unfold subst at 4. 
+    fold (subst tau p1). fold (subst tau p2). 
+    unfold subst at 3.
+    fold (subst sig (subst tau p1)). 
+    fold (subst sig (subst tau p2)).
+    rewrite H1. unfold compose at 1.
+    rewrite H2. unfold compose at 1. 
+  reflexivity.
 
-  clear phi. intros x p1 H1. unfold subst at 1. 
-  fold (subst (compose tau sig) p1).
+  clear phi. intros x p1 H1. 
+    unfold subst at 1. 
+    fold (subst (compose tau sig) p1).
+    unfold compose at 1. rewrite H1. unfold compose at 1.
+    unfold compose. unfold subst at 4. fold (subst tau p1).
+    unfold subst at 3. fold (subst sig (subst tau p1)).
+  reflexivity.
+Qed.
 
-Show.
+Definition identity {V:Set} (phi: V) := phi.
+
+Lemma subst_identity: forall V: Set, forall phi: P V,
+  subst identity phi = identity phi.
+Proof.
+  intros V phi. elim phi.
+
+  clear phi. intros x y.
+    unfold subst. unfold identity.
+  reflexivity.
+
+  clear phi. 
+    unfold subst. unfold identity.
+  reflexivity.
+
+  clear phi. intros p1 H1 p2 H2.
+    unfold subst. fold (subst identity p1). fold (subst identity p2).
+    rewrite H1, H2. unfold identity.
+  reflexivity.
+
+  clear phi. intros x p1 H1. 
+    unfold subst. fold (subst identity p1).
+    rewrite H1. unfold identity.
+  reflexivity.
+Qed. 
+
+
 
