assembly/64bits/att.sh
@@ -1,0 +1,34 @@
+#!/bin/sh
+
+# returns generated code for single at&t assembly instruction
+
+# e.g.
+# $ ./att.sh xor %rax, %rax
+# 48 31 c0 xor %rax,%rax
+
+# note that you need to escape '$' on input:
+# e.g.
+# $ ./att.sh movq \$2, %rax
+# 48 c7 c0 02 00 00 00 mov $0x2,%rax
+
+argument=$(echo "$@" | sed 's/att.sh/%/g' -)
+
+echo ".section .text" >  log.s
+echo ".global _start" >> log.s
+echo "_start:"        >> log.s 
+echo "$argument"      >> log.s
+echo "movq \$60,%rax" >> log.s
+echo "movq \$0, %rdi" >> log.s
+echo "syscall"        >> log.s
+
+as -o log.o log.s
+ld -o log log.o
+objdump -d log > log1
+
+for w in "$(cat log1 | grep -A1 _start | grep -v _start | cut -d':' -f2)"
+do
+  echo -n $w
+done
+echo
+
+rm -f log.s log.o log log1
