assembly/64bits/intel.sh
@@ -1,0 +1,31 @@
+#!/bin/sh
+
+# returns generated code for single intel assembly instruction
+
+# e.g.
+# $ ./intel.sh xor rax, rax
+# 48 31 c0 xor rax,rax
+
+# e.g.
+# $ ./intel.sh mov rax, 2
+# 48 c7 c0 02 00 00 00 mov rax,0x20 
+
+echo "segment .text"  >  log.asm
+echo "global _start"  >> log.asm
+echo "_start:"        >> log.asm 
+echo "$@"             >> log.asm
+echo "mov rax, 60"    >> log.asm
+echo "mov rdi, 0"     >> log.asm
+echo "syscall"        >> log.asm
+
+yasm -f elf64 log.asm
+ld -o log log.o
+objdump -d -M intel log > log1
+
+for w in "$(cat log1 | grep -A1 _start | grep -v _start | cut -d':' -f2)"
+do
+  echo -n $w
+done
+echo
+
+rm -f log.asm log.o log log1
