assembly/64bits/test.sh
@@ -10,14 +10,14 @@ cd ${HOME}
 ./hello/test.sh
 
 # intel syntax
-./yasm.sh exit.asm; ld exit.o; ./a.out; ./clean.sh             #_start
-./yasm.sh memory.asm; gcc memory.o; ./a.out; ./clean.sh        # main , no c lib
-./array_build.sh; ./array 20; ./clean.sh
 ./yasm.sh register.asm; ld register.o; ./a.out; ./clean.sh
-
 
 # at&t syntax
 ./as.sh  register.s; ld register.o; ./a.out; ./clean.sh
+
+# c++
+./yasm.sh ASMFunctions.asm;
+g++ -no-pie extern.cpp ASMFunctions.o; ./a.out; ./clean.sh
 
 
 cd ${DIR}
